remove some redundant code from GrammarAnalysis

GrammarAnalysis.v
@@ -41,6 +41,75 @@ Module GrammarAnalysisFn (Import D : Defs.T).
 
   Hint Constructors frame_step : core.
 
+  (* Correspondence between closure_multistep and frame_step relations *)
+  
+  Lemma closure_step__frame_step :
+    forall g av av' sp sp' pr pr' fr fr' frs frs',
+      sp     = Sp pr  (fr, frs)
+      -> sp' = Sp pr' (fr', frs')
+      -> suffix_stack_wf g (fr, frs)
+      -> closure_step g av sp av' sp'
+      -> frame_step g fr fr'.
+  Proof.
+    intros g av av' ? ? pr pr' fr fr' frs frs' ? ? hw hc; subst; inv hc; eauto.
+    - inv_suffix_frames_wf hw   hi  hw'  ; eauto.
+      inv_suffix_frames_wf hw'  hi' hw'' ; eauto.
+    - inv_suffix_frames_wf hw   hi  hw'  ; eauto.
+  Qed.
+
+  Lemma closure_multistep__frame_step_trc' :
+    forall g av av' sp sp',
+      suffix_stack_wf g (stack sp)
+      -> closure_multistep g av sp av' sp'
+      -> (forall pr pr' fr fr' frs frs',
+             sp     = Sp pr  (fr, frs)
+             -> sp' = Sp pr' (fr', frs')
+             -> clos_refl_trans_1n _ (frame_step g) fr fr').
+  Proof.
+    intros g av av' sp sp' hw hc. 
+    induct_cm hc hs hc' IH; intros pr pr' fr fr' ? ? heq heq'; subst; sis.
+    - inv heq; inv heq'; apply rt1n_refl.
+    - inv heq; inv heq'; apply rt1n_refl.
+    - pose proof hs as hs'.
+      inv hs'.
+      + (* return case *)
+        eapply closure_step__frame_step in hs; eauto.
+        inv hs.
+        * (* final return case *)
+          inv hw; rew_anr.
+          inv H7.
+          eapply rt1n_trans.
+          -- sis; eapply Fstep_final_ret; eauto.
+          -- eapply IH; eauto. sis; auto. 
+        * (* nonfinal return case *)
+          eapply rt1n_trans.
+          -- sis; eapply Fstep_nonfinal_ret; eauto.
+          -- eapply IH; eauto; sis.
+             eapply return_preserves_suffix_frames_wf_invar; eauto.
+      + (* push case *)
+        eapply closure_step__frame_step in hs; eauto; sis.
+        inv hs.
+        * eapply rt1n_trans; eauto.
+          eapply IH; eauto.
+          apply push_preserves_suffix_frames_wf_invar; auto.
+        * eapply rt1n_trans; eauto.
+          eapply IH; eauto.
+          apply push_preserves_suffix_frames_wf_invar; auto.
+  Qed.
+
+  Lemma closure_multistep__frame_step_trc :
+    forall g av av' sp sp' pr pr' fr fr' frs frs',
+      sp     = Sp pr  (fr, frs)
+      -> sp' = Sp pr' (fr', frs')
+      -> suffix_stack_wf g (stack sp)
+      -> closure_multistep g av sp av' sp'
+      -> clos_refl_trans_1n _ (frame_step g) fr fr'.
+  Proof.
+    intros; eapply closure_multistep__frame_step_trc'; eauto.
+  Qed.
+
+  (* COMPUTATION OF SINGLE-STEP FRAME CLOSURE EDGES *)
+
   Definition step_edges_sound (g : grammar) (es : list edge) :=
     forall x y, In (x, y) es -> frame_step g x y.
 
@@ -56,13 +125,18 @@ Module GrammarAnalysisFn (Import D : Defs.T).
   Definition mstep_edges_sound (g : grammar) (es : list edge) :=
     forall x y, In (x, y) es -> frame_multistep g x y.
 
+  Lemma step_edges_sound__mstep_edges_sound :
+    forall g es,
+      step_edges_sound g es -> mstep_edges_sound g es.
+  Proof.
+    intros g es hs s d hi; apply t_step; auto.
+  Qed.
+
   Definition mstep_edges_complete (g : grammar) (es : list edge) :=
     forall x y, frame_multistep g x y -> In (x, y) es.
 
   Definition mstep_edges_correct (g : grammar) (es : list edge) :=
     mstep_edges_sound g es /\ mstep_edges_complete g es.
-
-  (* COMPUTATION OF SINGLE-STEP FRAME CLOSURE EDGES *)
 
   Definition initialPushEdges' (g : grammar) (x : nonterminal) : list edge :=
     map (fun rhs => (SF None [NT x], SF (Some x) rhs))
@@ -289,196 +363,23 @@ Module GrammarAnalysisFn (Import D : Defs.T).
       eapply pushEdges_complete; eauto.
   Qed.
 
-  Lemma step_edges_sound__mstep_edges_sound :
-    forall g es,
-      step_edges_sound g es -> mstep_edges_sound g es.
-  Proof.
-    intros g es hs s d hi; apply t_step; auto.
-  Qed.
-
-  (* More efficient implementation of transClosure *)
-  Module FS' := FSetAVL.Make SF_as_UOT.
-  Module FSF' := FSetFacts.Facts FS'.
-  Module FM' <: FMapInterface.S := FMapAVL.Make SF_as_UOT.
-  Module FMF' := FMapFacts.Facts FM'.
-  Module TC  := TransClos.Make FS' FM'.
-
-  Lemma in_elements_iff_in_FS :
-    forall fr s,
-      In fr (FS'.elements s) <-> FS'.In fr s.
-  Proof.
-    intros fr s; split; intros hi.
-    - eapply FSF'.elements_iff.
-      eapply In_InA; eauto.
-    - eapply FSF'.elements_iff in hi. 
-      eapply InA_alt in hi; destruct hi as [fr' [heq hi]]; subst; auto.
-  Qed.
+  (* transitive closure operation *)
 
   Definition liftEdge (e : edge) : option (suffix_frame * list suffix_frame) :=
     match e with
     | (s, d) => Some (s, [d])
     end.
   
-  Definition transClos' (es : list edge) : FM'.t FS'.t :=
+  Definition transClos (es : list edge) : FM.t FS.t :=
     TC.trans_clos_list liftEdge es.
 
-  (* Now we keep only the "stable" edges *)
-
-  Definition stable (fr : suffix_frame) : bool :=
-    match fr with
-    | SF None []             => true
-    | SF _        (T _ :: _) => true
-    | _                      => false
-    end.
-
-  Lemma stable_compat_bool :
-    compat_bool eq stable.
-  Proof.
-    repeat red; intros; subst; auto.
-  Qed.
-
-  Lemma stable_config__stable_true :
-    forall fr frs,
-      stable_config (fr, frs)
-      -> stable fr = true.
-  Proof.
-    intros fr frs hs; inv hs; auto.
-    sis; dm; tc.
-  Qed.
-
-  Definition dstStable (e : edge) : bool :=
-    let (_, b) := e in stable b.
-
-  Definition stableEdges (es : list edge) : list edge :=
-    filter dstStable es.
-
-  Definition keepStableNodes (s : FS'.t) : list suffix_frame :=
-    FS'.elements (FS'.filter stable s).
-
-  Lemma keepStableNodes_stable :
-    forall fr frs,
-      In fr (keepStableNodes frs)
-      -> stable fr = true.
-  Proof.
-    intros fr frs hi.
-    unfold keepStableNodes in hi.
-    apply in_elements_iff_in_FS in hi.
-    eapply FS'.filter_2; eauto.
-    apply stable_compat_bool.
-  Qed.
-
-  (* A closure graph is a map where each key K is a suffix frame 
-     (i.e., grammar location), and each value V is a list of frames 
-     that are epsilon-reachable from K *)
-  (* Maybe the value should be a set *)
-  Definition closure_map := FM'.t (list suffix_frame).
-
-  Definition keepStableEdges (g : TC.G.graph) : closure_map :=
-    FM'.map keepStableNodes g.
-
-  Definition mkClosureMap (g : grammar) : closure_map :=
-    keepStableEdges (transClos' (epsilonEdges g)).
-
-  Definition destFrames (fr : suffix_frame) (cm : closure_map) : list suffix_frame :=
-    match FM'.find fr cm with
-    | Some frs => frs
-    | None     => []
-    end.
-
-  (* Correctness of grammar static analysis *)
-
-  Lemma closure_step__frame_step :
-    forall g av av' sp sp' pr pr' fr fr' frs frs',
-      sp     = Sp pr  (fr, frs)
-      -> sp' = Sp pr' (fr', frs')
-      -> suffix_stack_wf g (fr, frs)
-      -> closure_step g av sp av' sp'
-      -> frame_step g fr fr'.
-  Proof.
-    intros g av av' ? ? pr pr' fr fr' frs frs' ? ? hw hc; subst; inv hc; eauto.
-    - inv_suffix_frames_wf hw   hi  hw'  ; eauto.
-      inv_suffix_frames_wf hw'  hi' hw'' ; eauto.
-    - inv_suffix_frames_wf hw   hi  hw'  ; eauto.
-  Qed.
-
-  Lemma closure_multistep__frame_step_trc' :
-    forall g av av' sp sp',
-      suffix_stack_wf g (stack sp)
-      -> closure_multistep g av sp av' sp'
-      -> (forall pr pr' fr fr' frs frs',
-             sp     = Sp pr  (fr, frs)
-             -> sp' = Sp pr' (fr', frs')
-             -> clos_refl_trans_1n _ (frame_step g) fr fr').
-  Proof.
-    intros g av av' sp sp' hw hc. 
-    induct_cm hc hs hc' IH; intros pr pr' fr fr' ? ? heq heq'; subst; sis.
-    - inv heq; inv heq'; apply rt1n_refl.
-    - inv heq; inv heq'; apply rt1n_refl.
-    - pose proof hs as hs'.
-      inv hs'.
-      + (* return case *)
-        eapply closure_step__frame_step in hs; eauto.
-        inv hs.
-        * (* final return case *)
-          inv hw; rew_anr.
-          inv H7.
-          eapply rt1n_trans.
-          -- sis; eapply Fstep_final_ret; eauto.
-          -- eapply IH; eauto. sis; auto. 
-        * (* nonfinal return case *)
-          eapply rt1n_trans.
-          -- sis; eapply Fstep_nonfinal_ret; eauto.
-          -- eapply IH; eauto; sis.
-             eapply return_preserves_suffix_frames_wf_invar; eauto.
-      + (* push case *)
-        eapply closure_step__frame_step in hs; eauto; sis.
-        inv hs.
-        * eapply rt1n_trans; eauto.
-          eapply IH; eauto.
-          apply push_preserves_suffix_frames_wf_invar; auto.
-        * eapply rt1n_trans; eauto.
-          eapply IH; eauto.
-          apply push_preserves_suffix_frames_wf_invar; auto.
-  Qed.
-
-  Lemma closure_multistep__frame_step_trc :
-    forall g av av' sp sp' pr pr' fr fr' frs frs',
-      sp     = Sp pr  (fr, frs)
-      -> sp' = Sp pr' (fr', frs')
-      -> suffix_stack_wf g (stack sp)
-      -> closure_multistep g av sp av' sp'
-      -> clos_refl_trans_1n _ (frame_step g) fr fr'.
-  Proof.
-    intros; eapply closure_multistep__frame_step_trc'; eauto.
-  Qed.
-
-  Definition closure_map_sound g cm :=
-    forall fr fr' frs',
-      FM'.MapsTo fr frs' cm
-      -> In fr' frs'
-      -> (frame_multistep g fr fr' /\ stable fr' = true).
-
-  Definition closure_map_complete g cm :=
-    forall fr fr',
-      frame_multistep g fr fr'
-      -> stable fr' = true
-      -> exists frs',
-          FM'.MapsTo fr frs' cm
-          /\ In fr' frs'.
-
-  Definition closure_map_correct g cm :=
-    closure_map_sound g cm /\ closure_map_complete g cm.
+  (* soundness of transitive closure operation *)
 
   Definition tc_soundness_invar g cm :=
-    forall s d,
-      TC.G.rel cm s d
-      -> frame_multistep g s d.
+    forall s d, TC.G.rel cm s d -> frame_multistep g s d.
 
   Definition tc_soundness_invar_list g prs :=
-    forall s d ds,
-      In (s, ds) prs
-      -> FS'.In d ds
-      -> frame_multistep g s d.
+    forall s d ds, In (s, ds) prs -> FS.In d ds -> frame_multistep g s d.
 
   Lemma tc_soundness_invar_list_tail :
     forall g s ds prs,
@@ -490,13 +391,13 @@ Module GrammarAnalysisFn (Import D : Defs.T).
   Qed.
 
   Lemma in_elements_find_iff :
-    forall s (ds : FS'.t) cm,
-      In (s, ds) (FM'.elements cm)
-      <-> FM'.find s cm = Some ds.
+    forall s (ds : FS.t) cm,
+      In (s, ds) (FM.elements cm)
+      <-> FM.find s cm = Some ds.
   Proof.
     intros s ds cm; split; intros hi.
-    - apply FMF'.find_mapsto_iff.
-      apply FMF'.elements_mapsto_iff.
+    - apply FMF.find_mapsto_iff.
+      apply FMF.elements_mapsto_iff.
       apply In_InA; auto.
       (* lemma *)
       constructor.
@@ -504,8 +405,8 @@ Module GrammarAnalysisFn (Import D : Defs.T).
       + repeat red; intros x y he; destruct he; auto.
       + repeat red. intros (a, b) (c, d) (e, f) he he'; sis.
         repeat red in he, he'; sis; destruct he; destruct he'; subst; auto.
-    - apply FMF'.find_mapsto_iff in hi.
-      apply FM'.elements_1 in hi.
+    - apply FMF.find_mapsto_iff in hi.
+      apply FM.elements_1 in hi.
       apply InA_alt in hi.
       destruct hi as [(s', ds') [he hi]].
       repeat red in he; sis; destruct he; subst; auto.
@@ -513,7 +414,7 @@ Module GrammarAnalysisFn (Import D : Defs.T).
 
   Lemma invars_equiv :
     forall g cm,
-      tc_soundness_invar g cm <-> tc_soundness_invar_list g (FM'.elements cm).
+      tc_soundness_invar g cm <-> tc_soundness_invar_list g (FM.elements cm).
   Proof.
     intros g cm; split; intros hs.
     - intros s d ds hi hi'.
@@ -536,11 +437,11 @@ Module GrammarAnalysisFn (Import D : Defs.T).
     red; intros s' d' hr; red in hr.
     destruct hr as [ds' [hfi hin]].
     destruct (SF_as_UOT.eq_dec s' s) as [he | hn]; subst.
-    - rewrite FMF'.add_eq_o in hfi; auto; inv hfi.
+    - rewrite FMF.add_eq_o in hfi; auto; inv hfi.
       destruct (SF_as_UOT.eq_dec d' d) as [he' | hn']; subst; auto.
-      apply FS'.add_3 in hin; auto.
+      apply FS.add_3 in hin; auto.
       apply hs; apply TC.G.In_succs_rel; auto.
-    - rewrite FMF'.add_neq_o in hfi; auto.
+    - rewrite FMF.add_neq_o in hfi; auto.
       apply hs; red; eauto.
   Qed.
 
@@ -550,7 +451,7 @@ Module GrammarAnalysisFn (Import D : Defs.T).
       -> tc_soundness_invar g cm
       -> tc_soundness_invar g
                             (fold_left
-                               (fun (a : TC.G.graph) (e : FS'.elt) =>
+                               (fun a e =>
                                   TC.G.add_edge s e a)
                                ds cm).
   Proof.
@@ -559,33 +460,44 @@ Module GrammarAnalysisFn (Import D : Defs.T).
     apply add_edge_pres_soundness; auto.
   Qed.
 
+  Lemma in_elements_iff_in_FS :
+    forall fr s,
+      In fr (FS.elements s) <-> FS.In fr s.
+  Proof.
+    intros fr s; split; intros hi.
+    - eapply FSF.elements_iff.
+      eapply In_InA; eauto.
+    - eapply FSF.elements_iff in hi. 
+      eapply InA_alt in hi; destruct hi as [fr' [heq hi]]; subst; auto.
+  Qed.
+  
   Lemma in_elements_add :
     forall x y zs,
-      In x (FS'.elements (FS'.add y zs))
-      -> x = y \/ In x (FS'.elements zs).
+      In x (FS.elements (FS.add y zs))
+      -> x = y \/ In x (FS.elements zs).
   Proof.
     intros x y zs hi.
     apply in_elements_iff_in_FS in hi.
-    apply FSF'.add_iff in hi; destruct hi; auto.
+    apply FSF.add_iff in hi; destruct hi; auto.
     right; apply in_elements_iff_in_FS; auto.
   Qed.
 
   Lemma add_pred_preserves_soundness :
     forall g cm cm' s s' d ds',
       frame_multistep g s d
-      -> (forall d', FS'.In d' ds' -> frame_multistep g s' d')
+      -> (forall d', FS.In d' ds' -> frame_multistep g s' d')
       -> tc_soundness_invar g cm
       -> tc_soundness_invar g cm'
       -> tc_soundness_invar g
-                            (TC.add_pred s (FS'.add d (TC.G.succs d cm)) s' ds' cm').
+                            (TC.add_pred s (FS.add d (TC.G.succs d cm)) s' ds' cm').
   Proof.
     intros g cm cm' s s' d ds' hf ha hs hs'.
     unfold TC.add_pred; dmeq heq; auto.
-    rewrite FS'.fold_1; apply fold_add_edge_preserves_soundness; auto.
+    rewrite FS.fold_1; apply fold_add_edge_preserves_soundness; auto.
     intros d' hi.
     assert (hf' : frame_multistep g s' d).
     { eapply t_trans; eauto.
-      apply ha; apply FSF'.mem_iff; auto. }
+      apply ha; apply FSF.mem_iff; auto. }
     apply in_elements_add in hi; destruct hi as [? | hi]; subst; auto.
     eapply t_trans; eauto.
     apply hs; eauto.
@@ -601,8 +513,8 @@ Module GrammarAnalysisFn (Import D : Defs.T).
       -> tc_soundness_invar g cm'
       -> tc_soundness_invar g
                             (fold_left
-                               (fun (a : TC.G.graph) (p : FM'.key * FS'.t) =>
-                                  TC.add_pred s (FS'.add d (TC.G.succs d cm)) 
+                               (fun a p =>
+                                  TC.add_pred s (FS.add d (TC.G.succs d cm)) 
                                               (fst p) (snd p) a)
                                prs cm').
   Proof.
@@ -622,12 +534,11 @@ Module GrammarAnalysisFn (Import D : Defs.T).
   Proof.
     intros g cm s d hf hs.
     unfold TC.trans_add_edge; dm; auto.
-    rewrite FM'.fold_1.
+    rewrite FM.fold_1.
     apply fold_add_pred_preserves_tc_soundness_invar; auto.
     - apply invars_equiv; auto.
-    - (* adding the successors preserves soundness *)
-      (* lemma *)
-      rewrite FS'.fold_1; apply fold_add_edge_preserves_soundness; auto.
+    - (* lemma *)
+      rewrite FS.fold_1; apply fold_add_edge_preserves_soundness; auto.
       intros d' hi; apply in_elements_add in hi.
       destruct hi as [? | hi]; subst; auto.
       apply t_trans with (y := d); auto.
@@ -648,11 +559,11 @@ Module GrammarAnalysisFn (Import D : Defs.T).
       apply hs; apply in_eq.
   Qed.
 
-  Lemma transClos'_result_sound :
+  Lemma transClos_result_sound :
     forall g,
-      tc_soundness_invar g (transClos' (epsilonEdges g)).
+      tc_soundness_invar g (transClos (epsilonEdges g)).
   Proof.
-    intros g; unfold transClos', TC.trans_clos_list.
+    intros g; unfold transClos, TC.trans_clos_list.
     apply fold_trans_add_edge_preserves_tc_soundness_invar. 
     - apply step_edges_sound__mstep_edges_sound.
       apply epsilonEdges__step_edges_sound.
@@ -660,34 +571,10 @@ Module GrammarAnalysisFn (Import D : Defs.T).
       red. intros s d hr.
       red in hr.
       destruct hr as [ds [hf hi]].
-      rewrite FMF'.empty_o in hf; inv hf.
+      rewrite FMF.empty_o in hf; inv hf.
   Qed.
-    
-  Lemma mkClosureMap_sound :
-    forall g,
-      closure_map_sound g (mkClosureMap g).
-  Proof.
-    intros g s d ds hm hi; unfold mkClosureMap in hm.
-    split.
-    - (* lemma about keepStableEdges *)
-      assert (hex : exists ds',
-                 FM'.MapsTo s ds' (transClos' (epsilonEdges g))
-                 /\ FS'.In d ds').
-      { apply FMF'.map_mapsto_iff in hm.
-        destruct hm as [ds' [? hm]]; subst; eauto.
-        eexists; split; eauto.
-        unfold keepStableNodes in hi.
-        eapply in_elements_iff_in_FS in hi.
-        apply FSF'.filter_iff in hi.
-        - destruct hi; auto.
-        - repeat red; intros; subst; auto. }
-      destruct hex as [ds' [hm' hi']].
-      apply FMF'.find_mapsto_iff in hm'.
-      apply transClos'_result_sound; red; eauto.
-    - apply FMF'.map_mapsto_iff in hm.
-      destruct hm as [ds' [he hm]]; subst.
-      eapply keepStableNodes_stable; eauto.
-  Qed.
+
+  (* completeness of transitive closure operation *)
 
   Definition closure_map_complete_wrt_edges cm es :=
     forall x y, In (x, y) es -> TC.G.rel cm x y.
@@ -703,14 +590,14 @@ Module GrammarAnalysisFn (Import D : Defs.T).
     destruct (SF_as_UOT.eq_dec x' x) as [he | hn]; subst.
     - destruct (SF_as_UOT.eq_dec y' y) as [he' | hn']; subst.
       + eexists; split.
-        * rewrite FMF'.add_eq_o; auto.
-        * apply FS'.add_1; auto.
+        * rewrite FMF.add_eq_o; auto.
+        * apply FS.add_1; auto.
       + eexists; split.
-        * rewrite FMF'.add_eq_o; auto.
-        * apply FS'.add_2.
+        * rewrite FMF.add_eq_o; auto.
+        * apply FS.add_2.
           unfold TC.G.succs; rewrite hf; auto.
     - eexists; split; eauto.
-      rewrite FMF'.add_neq_o; auto.
+      rewrite FMF.add_neq_o; auto.
   Qed.
 
   Lemma add_edge_adds_edge :
@@ -719,8 +606,8 @@ Module GrammarAnalysisFn (Import D : Defs.T).
   Proof.
     intros x y cm; red; unfold TC.G.add_edge.
     eexists; split.
-    - rewrite FMF'.add_eq_o; eauto.
-    - apply FS'.add_1; auto.
+    - rewrite FMF.add_eq_o; eauto.
+    - apply FS.add_1; auto.
   Qed.
 
   Lemma trans_add_edge_preserves_cm_complete_invar :
@@ -750,26 +637,134 @@ Module GrammarAnalysisFn (Import D : Defs.T).
     apply trans_add_edge_preserves_cm_complete_invar; auto.
   Qed.
 
-  Lemma transClos'_holds_orig_edges :
+  Lemma transClos_holds_orig_edges :
     forall es x y,
       In (x, y) es
-      -> TC.G.rel (transClos' es) x y.
+      -> TC.G.rel (transClos es) x y.
   Proof.
     intros es x y hi.
-    unfold transClos', TC.trans_clos_list.
+    unfold transClos, TC.trans_clos_list.
     apply fold_trans_add_edge_list_keeps_old_edges with (pre := []); auto.
     red; intros x' y' hc; inv hc.
   Qed.
   
-  Lemma transClos'_complete :
+  Lemma transClos_complete :
     forall g s d,
       frame_multistep g s d
-      -> TC.G.rel (transClos' (epsilonEdges g)) s d.
+      -> TC.G.rel (transClos (epsilonEdges g)) s d.
   Proof.
     intros g s d hf; induction hf.
-    - apply transClos'_holds_orig_edges.
+    - apply transClos_holds_orig_edges.
       apply epsilonEdges__step_edges_complete; auto.
     - eapply TC.transitive_trans_clos_list; eauto.
+  Qed.
+  
+  (* After performing the transitive closure,
+     we keep only the "stable" edges *)
+
+  Definition stable (fr : suffix_frame) : bool :=
+    match fr with
+    | SF None []             => true
+    | SF _        (T _ :: _) => true
+    | _                      => false
+    end.
+
+  Lemma stable_compat_bool :
+    compat_bool eq stable.
+  Proof.
+    repeat red; intros; subst; auto.
+  Qed.
+
+  Lemma stable_config__stable_true :
+    forall fr frs,
+      stable_config (fr, frs)
+      -> stable fr = true.
+  Proof.
+    intros fr frs hs; inv hs; auto.
+    sis; dm; tc.
+  Qed.
+
+  Definition dstStable (e : edge) : bool :=
+    let (_, b) := e in stable b.
+
+  Definition stableEdges (es : list edge) : list edge :=
+    filter dstStable es.
+
+  Definition keepStableNodes (s : FS.t) : list suffix_frame :=
+    FS.elements (FS.filter stable s).
+
+  Lemma keepStableNodes_stable :
+    forall fr frs,
+      In fr (keepStableNodes frs)
+      -> stable fr = true.
+  Proof.
+    intros fr frs hi.
+    unfold keepStableNodes in hi.
+    apply in_elements_iff_in_FS in hi.
+    eapply FS.filter_2; eauto.
+    apply stable_compat_bool.
+  Qed.
+
+  (* A closure graph is a map where each key K is a suffix frame 
+     (i.e., grammar location), and each value V is a list of frames 
+     that are epsilon-reachable from K *)
+  Definition closure_map := FM.t (list suffix_frame).
+
+  Definition keepStableEdges (g : TC.G.graph) : closure_map :=
+    FM.map keepStableNodes g.
+  
+  Definition mkClosureMap (g : grammar) : closure_map :=
+    keepStableEdges (transClos (epsilonEdges g)).
+
+  Definition destFrames (fr : suffix_frame) (cm : closure_map) : list suffix_frame :=
+    match FM.find fr cm with
+    | Some frs => frs
+    | None     => []
+    end.
+
+  (* mkClosureMap spec and correctness proofs *)
+
+  Definition closure_map_sound g cm :=
+    forall fr fr' frs',
+      FM.MapsTo fr frs' cm
+      -> In fr' frs'
+      -> (frame_multistep g fr fr' /\ stable fr' = true).
+
+  Definition closure_map_complete g cm :=
+    forall fr fr',
+      frame_multistep g fr fr'
+      -> stable fr' = true
+      -> exists frs',
+          FM.MapsTo fr frs' cm
+          /\ In fr' frs'.
+
+  Definition closure_map_correct g cm :=
+    closure_map_sound g cm /\ closure_map_complete g cm.
+    
+  Lemma mkClosureMap_sound :
+    forall g,
+      closure_map_sound g (mkClosureMap g).
+  Proof.
+    intros g s d ds hm hi; unfold mkClosureMap in hm.
+    split.
+    - (* lemma about keepStableEdges *)
+      assert (hex : exists ds',
+                 FM.MapsTo s ds' (transClos (epsilonEdges g))
+                 /\ FS.In d ds').
+      { apply FMF.map_mapsto_iff in hm.
+        destruct hm as [ds' [? hm]]; subst; eauto.
+        eexists; split; eauto.
+        unfold keepStableNodes in hi.
+        eapply in_elements_iff_in_FS in hi.
+        apply FSF.filter_iff in hi.
+        - destruct hi; auto.
+        - repeat red; intros; subst; auto. }
+      destruct hex as [ds' [hm' hi']].
+      apply FMF.find_mapsto_iff in hm'.
+      apply transClos_result_sound; red; eauto.
+    - apply FMF.map_mapsto_iff in hm.
+      destruct hm as [ds' [he hm]]; subst.
+      eapply keepStableNodes_stable; eauto.
   Qed.
 
   Lemma mkClosureMap_complete :
@@ -778,15 +773,15 @@ Module GrammarAnalysisFn (Import D : Defs.T).
   Proof.
     intros g s d hf hs.
     unfold mkClosureMap.
-    apply transClos'_complete in hf.
+    apply transClos_complete in hf.
     red in hf.
     destruct hf as [ds [hf hi]].
-    exists (FS'.elements (FS'.filter stable ds)); split.
-    - apply FMF'.map_mapsto_iff.
+    exists (FS.elements (FS.filter stable ds)); split.
+    - apply FMF.map_mapsto_iff.
       exists ds; split; auto.
-      apply FMF'.find_mapsto_iff; auto.
+      apply FMF.find_mapsto_iff; auto.
     - apply in_elements_iff_in_FS.
-      apply FS'.filter_3; auto.
+      apply FS.filter_3; auto.
       apply stable_compat_bool.
   Qed.
     
